theories/interop/basics_constructions.v
@@ -7,9 +7,6 @@ From melocoton.ml_lang Require Import lang.
 From melocoton.c_interface Require Import defs notation.
 From melocoton.interop Require Import basics state.
 
-Global Notation MLval := ML_lang.val.
-Global Notation Cval := C_intf.val.
-
 Section ChiZetaConstruction.
 
 Definition lookup_reversed `{Countable A} {B} (m : gmap A B) (b : B) :=
@@ -550,26 +547,30 @@ Proof.
     eexists. econstructor; done.
 Qed.
 
-Lemma find_repr_roots θ roots privmem :
-   roots_are_live θ roots
- → dom privmem ## dom roots
- → exists mem, repr θ roots privmem mem.
+Lemma find_repr_roots θ roots :
+  roots_are_live θ roots →
+  ∃ memr, repr_roots θ roots memr.
 Proof.
-  revert privmem. unfold repr.
-  induction roots as [|l a roots_m Hin IH] using map_ind; intros privmem Hlive Hdisj.
-  - exists privmem, ∅. split_and!.
-    + econstructor.
-    + eapply map_disjoint_empty_r.
-    + by rewrite map_empty_union.
-  - destruct (IH privmem) as (mem1 & memr1 & Hrepr1 & Hdisj1 & Heq1).
-    1: { intros a1 w1 H1; eapply Hlive; rewrite lookup_insert_ne; first done.
-         intros ->; rewrite Hin in H1; congruence. }
-    1: rewrite dom_insert_L in Hdisj; set_solver.
-    destruct (find_repr_lval_vv θ a) as (w & Hw).
-    1: intros γ <-; eapply Hlive; apply lookup_insert.
-    exists (<[l:=Storing w]> mem1), (<[l:=Storing w]> memr1). split_and!.
-    + econstructor. 1: done. 1:done. 2: erewrite <- repr_roots_dom; last apply Hrepr1. all: by eapply not_elem_of_dom.
-    + apply map_disjoint_dom in Hdisj1. apply map_disjoint_dom.
-      rewrite dom_insert_L. rewrite dom_insert_L in Hdisj. set_solver.
-    + erewrite Heq1. now rewrite insert_union_l.
+  induction roots as [|l lv roots_m Hin IH] using map_ind; intros Hlive.
+  { exists ∅. constructor. }
+  { destruct IH as (memr & Hmemr).
+    { intros l' γ Hl'. destruct (decide (l = l')) as [->|]; first congruence.
+      eapply (Hlive l'). rewrite lookup_insert_ne //. }
+    destruct (find_repr_lval_vv θ lv) as (w & Hw).
+    { intros γ <-. eapply Hlive; eapply lookup_insert. }
+    exists (<[l:=Storing w]> memr). constructor; eauto.
+    { by eapply not_elem_of_dom. }
+    { erewrite <-repr_roots_dom; eauto. by eapply not_elem_of_dom. } }
+Qed.
+
+Lemma find_repr_mem θ roots privmem :
+  roots_are_live θ roots →
+  dom privmem ## dom roots →
+  ∃ mem, repr_mem θ roots privmem mem.
+Proof.
+  intros Hlive Hdisj.
+  destruct (find_repr_roots _ _ Hlive) as (memr & Hrepr).
+  exists (memr ∪ privmem). eexists. split_and!; eauto.
+  apply map_disjoint_dom. apply repr_roots_dom in Hrepr.
+  rewrite -Hrepr//.
 Qed.
