theories/interop/wp_boundary_laws.v
@@ -9,7 +9,7 @@ From transfinite.base_logic.lib Require Import ghost_map ghost_var.
 From iris.proofmode Require Import proofmode.
 From melocoton.c_interface Require Import defs resources.
 From melocoton.ml_lang Require Import lang lang_instantiation primitive_laws.
-From melocoton.interop Require Import weakestpre wp_utils hybrid_ghost_heap.
+From melocoton.interop Require Import weakestpre hybrid_ghost_heap roots.
 Import Wrap.
 
 (** lemmas to switch between the ML<->C state interp at a boundary *)
@@ -35,15 +35,7 @@ Lemma wrap_interp_c_to_ml ws ρc mem θ vs lvs :
 Proof using.
   iIntros (Hlv) "Hσ HGC Hnb #Hblk".
   iNamed "Hσ". iNamed "SIC". iNamed "HGC". simplify_eq. SI_GC_agree.
-
-  iAssert (⌜∀ k lv, roots_m !! k = Some lv →
-            ∃ w, mem !! k = Some (Storing w) ∧ repr_lval (θC ρc) lv w⌝)%I as "%Hroots".
-  1: { iIntros (kk vv Hroots).
-       iPoseProof (big_sepM_lookup with "GCrootspto") as "(%wr & Hwr & %Hw2)"; first done.
-       iExists wr. iSplit; last done. iApply (gen_heap_valid with "HσC Hwr"). }
-  apply map_Forall_lookup_2 in Hroots.
-  destruct (make_repr (θC ρc) roots_m mem) as [privmem Hpriv]; try done; [].
-
+  iDestruct (ROOTS_valid with "GCROOTS HσC") as %(privmem & Hrepr).
   iDestruct (hgh_export_ml_heap with "GCHGH")
     as (ζ' χ' ζfreeze) "(GCHGH & Hσ & %Hχ & %Hfrz & %Hζ)".
   iAssert (⌜Forall2 (is_val χ' ζfreeze) vs lvs⌝)%I as %Hval.
@@ -61,15 +53,12 @@ Proof using.
   iMod (ghost_var_update_halves with "Hnb SIbound") as "(Hb & SIbound)".
   iMod (ghost_var_update_halves with "GCζ SIζ") as "(GCζ & SIζ)".
   iMod (ghost_var_update_halves with "GCχ SIχ") as "(GCχ & SIχ)".
-  iMod (ghost_var_update_halves with "GCθ SIθ") as "(GCθ & SIθ)".
-  iMod (ghost_var_update_halves with "GCroots SIroots") as "(GCroots & SIroots)".
-  iMod (set_to_none with "HσC GCrootspto") as "(HσC & GCrootspto)"; first done.
+  iMod (ghost_var_update_halves with "GCrootss SIroots") as "(GCroots & SIroots)".
 
   iModIntro. iSplitR "SIbound"; last by iFrame "SIbound".
   rewrite /= /named. iFrame "Hσ".
   unfold private_state_interp, ML_state_interp, GC_remnant, named; cbn.
-  iFrame. iPureIntro.
-  destruct Hpriv as (mem_r & ->%repr_roots_dom & Hpriv2 & Hpriv3); by apply map_disjoint_dom.
+  iFrame. iExists _, _. by iFrame.
 Qed.
 
 Lemma wrap_interp_c_to_ml_out ow ρc mem θ ov olv :
@@ -111,7 +100,7 @@ Proof using.
   iIntros (Hml_to_c Hval Hrepre) "Hst Hb".
   destruct Hml_to_c as (ζσ & ζnewimm & HH).
   destruct HH as (Hmono & Hblocks & Hprivblocks & HζC & Hζdisj &
-                    Hstore & ? & ? & Hroots & ?).
+                    Hstore & ? & ? & Hroots & Hreprmem).
 
   iNamed "Hst". iNamed "SIML". iNamed "SIGCrem".
   iDestruct (hgh_dom_lstore_sub with "GCHGH") as %Hζsub.
@@ -119,7 +108,7 @@ Proof using.
   iMod (ghost_var_update_halves with "SIζ GCζ") as "(SIζ & GCζ)".
   iMod (ghost_var_update_halves with "SIχ GCχ") as "(SIχ & GCχ)".
   iMod (ghost_var_update_halves with "SIθ GCθ") as "(SIθ & GCθ)".
-  iMod (ghost_var_update_halves with "SIroots GCroots") as "(SIroots & GCroots)".
+  iMod (ghost_var_update_halves with "SIroots GCrootss") as "(SIroots & GCrootss)".
   apply map_disjoint_union_r in Hζdisj as [Hζdisj1 Hζdisj2].
   iMod (hgh_import_ml_interp _ _ _ _ (ζC ρc) with "GCHGH HσML") as "GCHGH"; eauto.
   (* TODO: use lstore_hybrid_repr in the opsem? *)
@@ -131,7 +120,8 @@ Proof using.
     { destruct Hmono as [?%subseteq_dom ?]. set_solver. }
     { eapply is_store_blocks_lstore_dom_sub; eauto. }
     { eapply is_private_blocks_dom_sub; eauto. } }
-  iMod (set_to_some with "HσCv GCrootspto") as "(HσCv & GCrootspto)"; first done.
+
+  iMod (ROOTS_update_θ with "GCROOTS HσCv") as "[GCROOTS HσCv]"; [by eauto..|].
   iDestruct (hgh_block_sim_of_vals _ _ _ vs lvs with "GCHGH") as "#Hsim"; first eassumption.
 
   iModIntro. iFrame "Hnb". rewrite /= /named.
